regex/Regex/Syntax/Parser/Test.lean
@@ -29,6 +29,11 @@ private def test (input : String) (expected : Ast) : Bool :=
 #guard test "(a)" (.group (.char 'a'))
 #guard test "(?:a)" (.char 'a')
 
+#guard test "(?i)a" (.concat (.flags true) (.char 'a'))
+#guard test "(?-i)a" (.concat (.flags false) (.char 'a'))
+#guard test "(?i:a)" (.group (.concat (.flags true) (.char 'a')))
+#guard test "(?-i:a)" (.group (.concat (.flags false) (.char 'a')))
+
 #guard test "^" (.anchor .start)
 #guard test "$" (.anchor .eos)
 #guard test "^abc$" (.concat (.concat (.concat (.concat (.anchor .start) (.char 'a')) (.char 'b')) (.char 'c')) (.anchor .eos))
